secp256k1: add precomputed table with w = 5

code/k256/Hacl.Impl.K256.PointMul.fst
@@ -34,6 +34,17 @@ let table_inv_w4 : BE.table_inv_t U64 15ul 16ul =
   BE.table_inv_precomp len ctx_len k l table_len
 
 
+inline_for_extraction noextract
+let table_inv_w5 : BE.table_inv_t U64 15ul 32ul =
+  [@inline_let] let len = 15ul in
+  [@inline_let] let ctx_len = 0ul in
+  [@inline_let] let k = mk_k256_concrete_ops in
+  [@inline_let] let l = 5ul in
+  [@inline_let] let table_len = 32ul in
+  assert_norm (pow2 (v l) == v table_len);
+  BE.table_inv_precomp len ctx_len k l table_len
+
+
 let point_mul out scalar q =
   let h0 = ST.get () in
   SE.exp_fw_lemma S.mk_k256_concrete_ops (point_eval h0 q) 256 (qas_nat h0 scalar) 4;
@@ -91,7 +102,7 @@ val point_mul_g_double_vartime_noalloc:
     out:point
   -> scalar1:qelem -> q1:point
   -> scalar2:qelem -> q2:point
-  -> table2:lbuffer uint64 (16ul *! 15ul) ->
+  -> table2:lbuffer uint64 (32ul *! 15ul) ->
   Stack unit
   (requires fun h ->
     live h out /\ live h scalar1 /\ live h q1 /\
@@ -102,7 +113,7 @@ val point_mul_g_double_vartime_noalloc:
 
     qas_nat h scalar1 < S.q /\ qas_nat h scalar2 < S.q /\
     point_inv h q1 /\ point_eval h q1 == S.g /\ point_inv h q2 /\
-    table_inv_w4 (as_seq h q2) (as_seq h table2))
+    table_inv_w5 (as_seq h q2) (as_seq h table2))
   (ensures fun h0 _ h1 -> modifies (loc out) h0 h1 /\
     point_inv h1 out /\
     S.to_aff_point (point_eval h1 out) ==
@@ -113,28 +124,29 @@ let point_mul_g_double_vartime_noalloc out scalar1 q1 scalar2 q2 table2 =
   [@inline_let] let len = 15ul in
   [@inline_let] let ctx_len = 0ul in
   [@inline_let] let k = mk_k256_concrete_ops in
-  [@inline_let] let l = 4ul in
-  [@inline_let] let table_len = 16ul in
+  [@inline_let] let l = 5ul in
+  [@inline_let] let table_len = 32ul in
   [@inline_let] let bLen = 4ul in
   [@inline_let] let bBits = 256ul in
-
+  assert_norm (pow2 (v l) == v table_len);
+  
   let h0 = ST.get () in
-  recall_contents precomp_basepoint_table_w4 precomp_basepoint_table_lseq_w4;
+  recall_contents precomp_basepoint_table_w5 precomp_basepoint_table_lseq_w5;
   let h1 = ST.get () in
-  precomp_basepoint_table_lemma_w4 ();
-  assert (table_inv_w4 (as_seq h1 q1) (as_seq h1 precomp_basepoint_table_w4));
-  assert (table_inv_w4 (as_seq h1 q2) (as_seq h1 table2));
+  precomp_basepoint_table_lemma_w5 ();
+  assert (table_inv_w5 (as_seq h1 q1) (as_seq h1 precomp_basepoint_table_w5));
+  assert (table_inv_w5 (as_seq h1 q2) (as_seq h1 table2));
 
   ME.mk_lexp_double_fw_tables len ctx_len k l table_len
-    table_inv_w4 table_inv_w4
+    table_inv_w5 table_inv_w5
     (BE.lprecomp_get_vartime len ctx_len k l table_len)
     (BE.lprecomp_get_vartime len ctx_len k l table_len)
     (null uint64) q1 bLen bBits scalar1 q2 scalar2
-    (to_const precomp_basepoint_table_w4) (to_const table2) out;
+    (to_const precomp_basepoint_table_w5) (to_const table2) out;
 
   SE.exp_double_fw_lemma S.mk_k256_concrete_ops
     (point_eval h0 q1) 256 (qas_nat h0 scalar1)
-    (point_eval h0 q2) (qas_nat h0 scalar2) 4
+    (point_eval h0 q2) (qas_nat h0 scalar2) 5
 
 
 [@CInline]
@@ -143,14 +155,15 @@ let point_mul_g_double_vartime out scalar1 scalar2 q2 =
   [@inline_let] let len = 15ul in
   [@inline_let] let ctx_len = 0ul in
   [@inline_let] let k = mk_k256_concrete_ops in
-  [@inline_let] let table_len = 16ul in
-
+  [@inline_let] let table_len = 32ul in
+  assert_norm (pow2 5 == v table_len);
+  
   let q1 = create 15ul (u64 0) in
   make_g q1;
 
   let table2 = create (table_len *! len) (u64 0) in
   PT.lprecomp_table len ctx_len k (null uint64) q2 table_len table2;
   let h = ST.get () in
-  assert (table_inv_w4 (as_seq h q2) (as_seq h table2));
+  assert (table_inv_w5 (as_seq h q2) (as_seq h table2));
   point_mul_g_double_vartime_noalloc out scalar1 q1 scalar2 q2 table2;
   pop_frame ()
